theories_multisorted/Experiments.v
@@ -1,0 +1,81 @@
+From Prototype Require Import MPrelude MSig.
+
+(*********************************************************************************)
+(** *** Level zero. *)
+(*********************************************************************************)
+
+Inductive ty : Type :=
+| var_ty : nat -> ty
+| arr : ty -> ty -> ty
+| all : ty -> ty.
+
+Inductive tm : Type :=
+| app : tm -> tm -> tm
+| tapp : tm -> ty -> tm
+| vt : vl -> tm
+
+with vl : Type :=
+| var_vl : nat -> vl
+| lam : ty -> tm -> vl
+| tlam : tm -> vl.
+
+Equations rename_ty (rty : ren) : ty -> ty :=
+rename_ty rty (var_ty i) := var_ty (rty i) ;
+rename_ty rty (arr t1 t2) := arr (rename_ty rty t1) (rename_ty rty t2) ;
+rename_ty rty (all t) := all (rename_ty (up_ren rty) t).
+
+Equations rename_tm (rty : ren) (rvl : ren) : tm -> tm :=
+rename_tm rty rvl (app t1 t2) := app (rename_tm rty rvl t1) (rename_tm rty rvl t2) ;
+rename_tm rty rvl (tapp t1 t2) := tapp (rename_tm rty rvl t1) (rename_ty rty t2) ;
+rename_tm rty rvl (vt v) := vt (rename_vl rty rvl v)
+
+with rename_vl (rty : ren) (rvl : ren) : vl -> vl :=
+rename_vl rty rvl (var_vl i) := var_vl (rvl i) ;
+rename_vl rty rvl (lam t1 t2) := lam (rename_ty rty t1) (rename_tm rty (up_ren rvl ) t2) ;
+rename_vl rty rvl (tlam t) := tlam (rename_tm (up_ren rty) rvl t).
+
+
+
+(*********************************************************************************)
+(** *** Level one. *)
+(*********************************************************************************)
+
+Section Sec.
+Context (sig : signature).
+
+(** [occurs_aux] *)
+
+Inductive occurs_aux (s : fin nsort) : @arg_ty nbase nsort -> Prop :=
+| occurs_aux_term : occurs_aux s (AT_term s)
+| occurs_aux_bind {s' ty} : occurs_aux s ty -> occurs_aux s (AT_bind s' ty).
+
+Equations occurs_auxb : fin nsort -> @arg_ty nbase nsort -> bool :=
+occurs_auxb s (AT_base _) := false ;
+occurs_auxb s (AT_term s') := eqb_fin s s' ;
+occurs_auxb s (AT_bind _ ty) := occurs_auxb s ty.
+
+Lemma occurs_aux_spec s ty : reflect (occurs_aux s ty) (occurs_auxb s ty).
+Proof. Admitted.
+
+(** [occurs] *)
+
+Equations fin_existsb (n : nat) (P : fin n -> bool) : bool :=
+fin_existsb 0 _ := false ;
+fin_existsb (S n) P := P finO || fin_existsb n (fun i => P (finS i)).
+
+Definition occurs (s s' : fin nsort) : Prop :=
+  exists c : fin (nctor s'), Exists (occurs_aux s) (ctor_type c).
+
+Definition occursb (s s' : fin nsort) : bool :=
+  fin_existsb (nctor s') (fun c => existsb (occurs_auxb s) (ctor_type c)).
+  
+Lemma occurs_spec s s' : reflect (occurs s s') (occursb s s').
+Proof. Admitted. 
+
+(* TODO: transitive closure of [occurs]. *)
+
+(** [binds_aux] *)
+
+Inductive binds_aux (s : fin nsort) : @arg_ty nbase nsort -> Prop :=
+| binds_aux_base {ty} : binds_aux s (AT_bind s ty)
+| binds_aux_step {s' ty} : binds_aux s ty -> binds_aux s (AT_bind s' ty).
