theories_multisorted/MSig.v
@@ -1,0 +1,38 @@
+From Prototype Require Import MPrelude.
+
+(** This file defines the notion of abstract signature of a language. *)
+
+(** Argument types over a set of base types and a set of sorts. *)
+Inductive arg_ty {nbase nsort} :=
+| AT_base : fin nbase -> arg_ty
+| AT_term : fin nsort -> arg_ty
+| AT_bind : fin nsort -> arg_ty -> arg_ty.
+Derive NoConfusion NoConfusionHom for arg_ty.
+
+(** Kind of an expression (this is used in both level one and level two). *)
+Inductive kind {nbase nsort} := 
+| (** Term. *)
+  Kt : fin nsort -> kind
+| (** Constructor argument. *)
+  Ka : @arg_ty nbase nsort -> kind.
+Derive NoConfusion NoConfusionHom for kind.
+
+(** Signatures for abstract terms. *)
+Record signature :=
+{ nbase : nat 
+; base_type : fin nbase -> Type
+; nsort : nat 
+; nctor : fin nsort -> nat
+; ctor_type : forall s, fin (nctor s) -> list (@arg_ty nbase nsort) }.
+
+(** Most of the time we can omit writing the precise signature,
+    it will be inferred by typeclass resolution. *)
+Existing Class signature.
+
+(** Set the [signature] argument of the projections to be implicit. *)
+Arguments nbase {_}.
+Arguments base_type {_}.
+Arguments nsort {_}.
+Arguments nctor {_}.
+Arguments ctor_type {_ _}.
+
